wip mutable local arrays

pulse/lib/steel/pulse/Pulse.Reflection.Util.fst
@@ -22,6 +22,7 @@ let unit_fv = R.pack_fv unit_lid
 let unit_tm = R.pack_ln (R.Tv_FVar unit_fv)
 let bool_fv = R.pack_fv bool_lid
 let bool_tm = R.pack_ln (R.Tv_FVar bool_fv)
+let nat_lid = ["Prims"; "nat"]
 
 let tuple2_lid = ["FStar"; "Pervasives"; "Native"; "tuple2"]
 let fst_lid = ["FStar"; "Pervasives"; "Native"; "fst"]
@@ -538,7 +539,6 @@ let mk_rewrite (p q:R.term) =
   let t = pack_ln (Tv_App t (q, Q_Explicit)) in
   pack_ln (Tv_App t (`(), Q_Explicit))
 
-
 let mk_withlocal (ret_u:R.universe) (a init pre ret_t post body:R.term) =
   let open R in
   let lid = mk_pulse_lib_reference_lid "with_local" in
@@ -600,3 +600,55 @@ let mk_pts_to (a:R.term) (r:R.term) (perm:R.term) (v:R.term) : R.term =
 let full_perm_tm : R.term =
   let open R in
   pack_ln (Tv_FVar (pack_fv full_perm_lid))
+
+let pulse_lib_array_core = ["Pulse"; "Lib"; "Array"; "Core"]
+let mk_pulse_lib_array_core_lid s = pulse_lib_array_core @ [s]
+
+let array_lid = mk_pulse_lib_array_core_lid "array"
+let array_pts_to_lid = mk_pulse_lib_array_core_lid "pts_to"
+let array_length_lid = mk_pulse_lib_array_core_lid "length"
+let array_is_full_lid = mk_pulse_lib_array_core_lid "is_full_array"
+
+let mk_array (a:R.term) : R.term =
+  let open R in
+  let t = pack_ln (Tv_FVar (pack_fv array_lid)) in
+  pack_ln (Tv_App t (a, Q_Explicit))
+
+let mk_array_length (a:R.term) (arr:R.term) : R.term =
+  let open R in
+  let t = pack_ln (Tv_FVar (pack_fv array_length_lid)) in
+  let t = pack_ln (Tv_App t (a, Q_Implicit)) in
+  pack_ln (Tv_App t (arr, Q_Explicit))
+
+let mk_array_pts_to (a:R.term) (arr:R.term) (perm:R.term) (v:R.term) : R.term =
+  let open R in
+  let t = pack_ln (Tv_FVar (pack_fv array_pts_to_lid)) in
+  let t = pack_ln (Tv_App t (a, Q_Implicit)) in
+  let t = pack_ln (Tv_App t (arr, Q_Explicit)) in
+  let t = pack_ln (Tv_App t (perm, Q_Implicit)) in
+  pack_ln (Tv_App t (v, Q_Explicit))
+
+let mk_array_is_full (a:R.term) (arr:R.term) : R.term =
+  let open R in
+  let t = pack_ln (Tv_FVar (pack_fv array_is_full_lid)) in
+  let t = pack_ln (Tv_App t (a, Q_Implicit)) in
+  pack_ln (Tv_App t (arr, Q_Explicit))
+
+let mk_seq_create (a:R.term) (len:R.term) (v:R.term) : R.term =
+  let open R in
+  let t = pack_ln (Tv_FVar (pack_fv ["FStar"; "Seq"; "create"])) in
+  let t = pack_ln (Tv_App t (a, Q_Implicit)) in
+  let t = pack_ln (Tv_App t (len, Q_Explicit)) in
+  pack_ln (Tv_App t (v, Q_Explicit))
+
+let mk_withlocalarray (ret_u:R.universe) (a init len pre ret_t post body:R.term) =
+  let open R in
+  let lid = mk_pulse_lib_array_core_lid "with_local" in
+  let t = pack_ln (Tv_UInst (R.pack_fv lid) [ret_u]) in
+  let t = pack_ln (Tv_App t (a, Q_Implicit)) in
+  let t = pack_ln (Tv_App t (init, Q_Explicit)) in
+  let t = pack_ln (Tv_App t (len, Q_Explicit)) in
+  let t = pack_ln (Tv_App t (pre, Q_Implicit)) in
+  let t = pack_ln (Tv_App t (ret_t, Q_Implicit)) in
+  let t = pack_ln (Tv_App t (post, Q_Implicit)) in
+  pack_ln (Tv_App t (body, Q_Explicit))
