pulse/lib/steel/pulse/Pulse.Elaborate.Core.fst
@@ -261,6 +261,19 @@ let rec elab_st_typing (#g:env)
       let rbody = mk_abs (mk_ref ra) R.Q_Explicit rbody in
       mk_withlocal rret_u ra rinit rpre rret_t rpost rbody
 
+    | T_WithLocalArray _ init len _ init_t c x _ _ _ _ body_typing ->
+      let rret_u = comp_u c in
+      let ra = elab_term init_t in
+      let rinit = elab_term init in
+      let rlen = elab_term len in
+      let rret_t = elab_term (comp_res c) in
+      let rpre = elab_term (comp_pre c) in
+      let rpost = mk_abs rret_t R.Q_Explicit (elab_term (comp_post c)) in
+      let rbody = elab_st_typing body_typing in
+      let rbody = RT.close_term rbody x in
+      let rbody = mk_abs (mk_ref ra) R.Q_Explicit rbody in
+      mk_withlocalarray rret_u ra rinit rlen rpre rret_t rpost rbody
+
     | T_Admit _ {u;res;pre;post} c _ ->
       let ru = u in
       let rres = elab_term res in
