pulse/lib/steel/pulse/Pulse.Syntax.Naming.fsti
@@ -125,6 +125,12 @@ let rec freevars_st (t:st_term)
                 (Set.union (freevars initializer)
                            (freevars_st body))
 
+    | Tm_WithLocalArray { binder; initializer; length; body } ->
+      Set.union (freevars binder.binder_ty)
+                (Set.union (freevars initializer)
+                           (Set.union (freevars length)
+                                      (freevars_st body)))
+
     | Tm_Rewrite { t1; t2 } ->
       Set.union (freevars t1) (freevars t2)
 
@@ -266,6 +272,12 @@ let rec ln_st' (t:st_term) (i:int)
     | Tm_WithLocal { binder; initializer; body } ->
       ln' binder.binder_ty i &&
       ln' initializer i &&
+      ln_st' body (i + 1)
+
+    | Tm_WithLocalArray { binder; initializer; length; body } ->
+      ln' binder.binder_ty i &&
+      ln' initializer i &&
+      ln' length i &&
       ln_st' body (i + 1)
 
     | Tm_Rewrite { t1; t2 } ->
@@ -509,6 +521,12 @@ let rec subst_st_term (t:st_term) (ss:subst)
       Tm_WithLocal { binder = subst_binder binder ss;
                      initializer = subst_term initializer ss;
                      body = subst_st_term body (shift_subst ss) }
+
+    | Tm_WithLocalArray { binder; initializer; length; body } ->
+      Tm_WithLocalArray { binder = subst_binder binder ss;
+                          initializer = subst_term initializer ss;
+                          length = subst_term length ss;
+                          body = subst_st_term body (shift_subst ss) }
 
     | Tm_Rewrite { t1; t2 } ->
       Tm_Rewrite { t1 = subst_term t1 ss;
