pulse/lib/steel/pulse/Pulse.Typing.FV.fst
@@ -184,6 +184,12 @@ let rec freevars_close_st_term' (t:st_term) (x:var) (i:index)
       freevars_close_term' initializer x i;
       freevars_close_st_term' body x (i + 1)
 
+    | Tm_WithLocalArray { binder; initializer; length; body } ->
+      freevars_close_term' binder.binder_ty x i;
+      freevars_close_term' initializer x i;
+      freevars_close_term' length x i;
+      freevars_close_st_term' body x (i + 1)
+
     | Tm_Admit { typ; post } ->
       freevars_close_term' typ x i;
       freevars_close_term_opt' post x (i + 1)
@@ -407,6 +413,10 @@ let freevars_ref (t:term)
   : Lemma (freevars (mk_ref t) == freevars t)
   = admit()
 
+let freevars_array (t:term)
+  : Lemma (freevars (mk_array t) == freevars t)
+  = admit()
+
 // FIXME: tame this proof
 #push-options "--fuel 2 --ifuel 1 --z3rlimit_factor 10 --query_stats --retry 5"
 let rec st_typing_freevars (#g:_) (#t:_) (#c:_)
@@ -581,6 +591,15 @@ let rec st_typing_freevars (#g:_) (#t:_) (#c:_)
      comp_typing_freevars c_typing;
      tot_or_ghost_typing_freevars u_typing;
      freevars_ref init_t
+
+   | T_WithLocalArray _ init len body init_t c x init_typing len_typing u_typing c_typing body_typing ->
+     tot_or_ghost_typing_freevars init_typing;
+     tot_or_ghost_typing_freevars len_typing;
+     st_typing_freevars body_typing;
+     freevars_open_st_term_inv body x;
+     comp_typing_freevars c_typing;
+     tot_or_ghost_typing_freevars u_typing;
+     freevars_array init_t
 
    | T_Admit _ s _ (STC _ _ x t_typing pre_typing post_typing) ->
      tot_or_ghost_typing_freevars t_typing;
